Added WIP proof showing a valid colouring preserves code behaviour

three_addrScript.sml
@@ -10,12 +10,23 @@ val _ = new_theory "three_addr";
 val _ = Hol_datatype `
   inst = Inst of num => num => num `
 
+(* type of colouring *)
+
+val _ = Hol_datatype `
+  colouring = Col of num => num`
+
 (* semantics of instruction evaluation *)
 
 val eval_def = Define `
   (eval f s [] = s) /\
   (eval f s ((Inst w r1 r2)::code) =
      eval f ((w =+ f (s r1) (s r2)) s) code)`;
+
+(* apply a colouring to a set of instructions *)
+val apply_def = Define `
+    (apply c [] = []) /\
+    (apply c ((Inst w r1 r2)::code) = (Inst (c w) (c r1) (c r2))::(apply c code))
+`
 
 (* helper functions *)
 
@@ -39,6 +50,7 @@ val get_live_def = Define `
   (get_live [] live = live) /\
   (get_live ((Inst w r1 r2)::code) live =
      insert r1 (insert r2 (delete w (get_live code live))))`;
+
 
 (* test *)
 
@@ -103,5 +115,130 @@ THEN1 (
   ]
 )
 );
+
+
+
+val duplicate_free_def = Define `
+    (duplicate_free [] = T) /\
+    (duplicate_free (x::xs) = ~(MEM x xs) /\ duplicate_free xs)
+`
+
+val colouring_ok_def = Define `
+    (colouring_ok c code live = duplicate_free (MAP c (get_live code live)))
+`
+
+
+val no_dead_code_def = Define `
+    (no_dead_code [] _ = T) /\
+    (no_dead_code ((Inst w r1 r2)::code) live = MEM w (get_live code live)
+    		  /\ no_dead_code code live)
+`
+
+
+val duplicate_free_map = prove(
+``
+duplicate_free (MAP c list) ==> duplicate_free (list)
+``,
+REPEAT STRIP_TAC THEN
+Induct_on `list` THEN1 (
+EVAL_TAC)
+THEN1 (
+STRIP_TAC THEN
+STRIP_TAC THEN
+FULL_SIMP_TAC bool_ss [MAP] THEN
+`duplicate_free (MAP c list)` by (FULL_SIMP_TAC bool_ss [duplicate_free_def]) THEN
+`duplicate_free list` by METIS_TAC [] THEN
+FULL_SIMP_TAC bool_ss [duplicate_free_def] THEN
+Cases_on `MEM h list` THEN1 (
+FULL_SIMP_TAC bool_ss [MEM] THEN
+cheat) (* todo - is sort-of trivial but hard *)
+THEN1 (METIS_TAC [])))
+
+
+(* Lemma for the below, need to do something for deletion too *)
+val duplicate_free_map_insertion = prove(``
+    duplicate_free (MAP c (insert n x)) ==>
+    duplicate_free (MAP c x)
+``,
+EVAL_TAC THEN STRIP_TAC THEN Cases_on `MEM n x`
+THEN1 (FULL_SIMP_TAC bool_ss [])
+THEN1 (FULL_SIMP_TAC bool_ss []
+      THEN FULL_SIMP_TAC bool_ss [MAP, duplicate_free_def]))
+
+(* need this to obtain `colouring_ok c code live` for the proof later *)
+``
+no_dead_code (Inst n n0 n1 :: code) live /\
+colouring_ok c (Inst n n0 n1 :: code) live ==>
+colouring_ok c code live
+``
+SIMP_TAC bool_ss [colouring_ok_def]
+SIMP_TAC bool_ss [get_live_def]
+STRIP_TAC
+`duplicate_free (MAP c (delete n (get_live code live)))`
+by METIS_TAC [duplicate_free_map_insertion]
+FULL_SIMP_TAC bool_ss [delete_def]
+(* TODO looks true but need to remove the `delete n`... *)
+
+
+
+(* no_dead_code is preserved by removing the first instruction *)
+val no_dead_code_preserved = prove(``
+    no_dead_code (Inst n n0 n1 :: code) live ==>
+    no_dead_code code live``,
+    RW_TAC std_ss [no_dead_code_def])
+
+
+``
+ !code s t c live f.
+    colouring_ok c code live /\ no_dead_code code live /\
+    (MAP s (get_live code live) = MAP (t o c) (get_live code live)) ==>
+    (MAP (eval f s code) live = MAP (eval f t (apply c code) o c) live)
+``
+Induct_on `code`
+EVAL_TAC THEN DECIDE_TAC
+
+FULL_SIMP_TAC std_ss []
+REPEAT STRIP_TAC
+Cases_on `h`
+EVAL_TAC
+(* plan: use the inductive lemma with appropriate substitutions for s and t.
+This will require transforming the conditions colouring_ok, no_dead_code etc.
+which work on (Inst n n0 n1 :: code) into ones working on code alone. *)
+
+
+(* Other proof idea: use eval_get_live?
+Gives us MAP (eval f s code) live = MAP (eval f (t o c) code) live
+Can the RHS of that be rewritten to MAP (eval f t (apply c code) o c) live
+as needed?
+We have that c is ok so applying c to live doesn't conflate things
+Looking at definitions of eval and apply, it looks like the equality should
+be valid maybe *)
+
+(* attempting the rewrite needed *)
+``
+! t c live f.
+MAP (eval f (t o c) code) live = MAP (eval f t (apply c code) o c) live
+``
+Induct_on `code`
+EVAL_TAC
+DECIDE_TAC
+Cases_on `h`
+RW_TAC bool_ss [apply_def]
+RW_TAC bool_ss [eval_def]
+(* This looks potentially right. Need to rearrange the ((n =+ blah) o (t o c))
+to a modification of t compatible with the one it needs to be equal to so we
+can use the inductive hypothesis.
+Would be roughly this:
+(c n =+ x) (t o c) = ((n =+ x) t) o c
+*)
+
+``
+! c n x t .
+(c n =+ x) (t o c) = ((n =+ x) t) o c
+``
+RW_TAC bool_ss [o_DEF]
+RW_TAC bool_ss [UPDATE_def]
+(* Have to prove the functions are equal - can this be broken down into showing
+they're equal for an arbitrary argument? *)
 
 val _ = export_theory();
